<?xml version="1.0"?>
<rdf:RDF xmlns="http://dveivr.dha.health.mil/transformations/2016/8/definitions#"
     xml:base="http://www.semanticweb.org/phoehne/ontologies/2016/8/definitions"
     xmlns:rdf="http://www.w3.org/1999/02/22-rdf-syntax-ns#"
     xmlns:owl="http://www.w3.org/2002/07/owl#"
     xmlns:xml="http://www.w3.org/XML/1998/namespace"
     xmlns:xsd="http://www.w3.org/2001/XMLSchema#"
     xmlns:rdfs="http://www.w3.org/2000/01/rdf-schema#">
    <owl:Ontology rdf:about="http://dveivr.dha.health.mil/transformations/2016/8/definitions"/>



    <!--
   ///////////////////////////////////////////////////////////////////////////////////////
   //
   // Classes
   //
   ///////////////////////////////////////////////////////////////////////////////////////
    -->

    <!-- http://dveivr.dha.health.mil/transformations/2016/8/definitions#SourceData -->
    <owl:Class rdf:about="http://dveivr.dha.health.mil/transformations/2016/8/definitions#DataSet">
        <rdfs:comment>This represents an existing data source.</rdfs:comment>
    </owl:Class>


    <!-- http://dveivr.dha.health.mil/transformations/2016/8/definitions#IngestTransformation -->

    <owl:Class rdf:about="http://dveivr.dha.health.mil/transformations/2016/8/definitions#IngestTransformation">
        <rdfs:comment>An individual transformation.  For example, the value &quot;YES&quot; for a given transformation
            mapps to &quot;http://some-uri.mil/my-ontology/an-attribute/some-value&quot;.</rdfs:comment>
    </owl:Class>



    <!-- http://dveivr.dha.health.mil/transformations/2016/8/definitions#InvokeTransformMapping -->

    <owl:Class rdf:about="http://dveivr.dha.health.mil/transformations/2016/8/definitions#InvokeTransformMapping">
        <rdfs:subClassOf rdf:resource="http://www.semanticweb.org/phoehne/ontologies/2016/8/transformations#Mapping"/>
        <rdfs:comment>This invokes a function in a module.  It refers to the URI of the module and the function name.
            The data from the source XML document and the XML document are passed to the function and the function
            output is used as the value.  For example, a function may translate an input value but would need to
            examine other XML document elements to determine the correct output value.  E.g. an element called &quot;
            last event date&quot; might require looking at the original XML to determine wha type of event is
            referenced.</rdfs:comment>
    </owl:Class>



    <!-- http://dveivr.dha.health.mil/transformations/2016/8/definitions#Mapping -->

    <owl:Class rdf:about="http://dveivr.dha.health.mil/transformations/2016/8/definitions#Mapping">
        <rdfs:comment>This is the root element for a data mapping, which allows the transformation from a value in
            the XML represenation of a patient/encounter/physician, etc. to a value in a triple.</rdfs:comment>
    </owl:Class>



    <!-- http://dveivr.dha.health.mil/transformations/2016/8/definitions#PassthroughValueMapping -->

    <owl:Class rdf:about="http://dveivr.dha.health.mil/transformations/2016/8/definitions#PassthroughValueMapping">
        <rdfs:subClassOf rdf:resource="http://dveivr.dha.health.mil/transformations/2016/8/definitions#Mapping"/>
        <rdfs:comment>A passthrough mapping takes the value found in the source XML document and copies it to the
            output triple without any transformation.  So if the element value in the source documents is &quot;foo&quot;,
            then the value in the output predicate is &quot;foo&quot;.</rdfs:comment>
    </owl:Class>



    <!-- http://dveivr.dha.health.mil/transformations/2016/8/definitions#SimpleValueMapping -->

    <owl:Class rdf:about="http://dveivr.dha.health.mil/transformations/2016/8/definitions#SimpleValueMapping">
        <rdfs:subClassOf rdf:resource="http://dveivr.dha.health.mil/transformations/2016/8/definitions#Mapping"/>
        <rdfs:comment>
            This performs a simple value mapping.  It is translating an input string to some output string.
            For example, the XML element may contain the words &quot;yes,&quot; &quot;no,&quot; or be null.  Those would translate
            to &quot;true&quot; or &quot;false.&quot;  Or, for exmple, having an input value as &quot;yes&quot; may translate into the
            URI of a class.  (E.g. if the value of the &quot;service-separated&quot; element in the XML document is &quot;yes&quot;,
            then that maps to the &quot;http://.../ServiceSeparated&quot; class.
        </rdfs:comment>
    </owl:Class>

    <!-- http://dveivr.dha.health.mil/transformations/2016/8/definitions#DefaultValue -->
    <owl:Class rdf:about="http://dveivr.dha.health.mil/transformations/2016/8/definitions#Parameter">
        <rdfs:comment>
            This provides the ability to associate default values with a transformation.  It will be used to
            pass values to the transformer functions.
        </rdfs:comment>
    </owl:Class>

    <!-- 
    ///////////////////////////////////////////////////////////////////////////////////////
    //
    // Object Properties
    //
    ///////////////////////////////////////////////////////////////////////////////////////
     -->

    <!-- http://www.semanticweb.org/phoehne/ontologies/2016/8/transformations#transformations -->

    <owl:ObjectProperty rdf:about="http://dveivr.dha.health.mil/transformations/2016/8/definitions#transformations">
        <rdfs:domain rdf:resource="http://dveivr.dha.health.mil/transformations/2016/8/definitions#IngestTransformation"/>
        <rdfs:range rdf:resource="http://dveivr.dha.health.mil/transformations/2016/8/definitions#Mapping"/>
        <rdfs:comment>This links an ingest transformation to all the data mappings.</rdfs:comment>
    </owl:ObjectProperty>

    <owl:ObjectProperty rdf:about="http://dveivr.dha.health.mil/transformations/2016/8/definitions#parameters">
        <rdfs:domain rdf:resource="http://dveivr.dha.health.mil/transformations/2016/8/definitions#InvokeTransformMapping"/>
        <rdfs:range rdf:resource="http://dveivr.dha.health.mil/transformations/2016/8/definitions#Parameter"/>
        <rdfs:comment>
            Links a function invocation to parameter values for the transformation function.  For example, a function
            might reformat a number, with the paramaters providing the format argument.
        </rdfs:comment>
    </owl:ObjectProperty>

    <owl:ObjectProperty rdf:about="http://dveivr.dha.health.mil/transformations/2016/8/definitions#associatedDataset">
        <rdfs:domain rdf:resource="http://dveivr.dha.health.mil/transformations/2016/8/definitions#IngestTransformation"/>
        <rdfs:range rdf:resource="http://dveivr.dha.health.mil/transformations/2016/8/definitions#DataSet"/>
        <rdfs:comment>Allows the transformation to indicate what dataset is applicable.</rdfs:comment>
    </owl:ObjectProperty>
    


    <!-- 
    ///////////////////////////////////////////////////////////////////////////////////////
    //
    // Data properties
    //
    ///////////////////////////////////////////////////////////////////////////////////////
     -->

    <!-- http://www.semanticweb.org/phoehne/ontologies/2016/8/transformations#collectionUri -->

    <owl:DatatypeProperty rdf:about="http://dveivr.dha.health.mil/transformations/2016/8/definitions#collectionUri">
        <rdfs:domain rdf:resource="http://dveivr.dha.health.mil/transformations/2016/8/definitions#DataSet"/>
        <rdfs:range rdf:resource="http://www.w3.org/2001/XMLSchema#anyURI"/>
        <rdfs:comment>
            This is the URI of the collection to which the data set definition refers.  For example, the patients
            data set has the "patient" collection.
        </rdfs:comment>
    </owl:DatatypeProperty>

    <!-- http://www.semanticweb.org/phoehne/ontologies/2016/8/transformations#lastExecuted -->

    <owl:DatatypeProperty rdf:about="http://dveivr.dha.health.mil/transformations/2016/8/definitions#executedOn">
        <rdfs:domain rdf:resource="http://dveivr.dha.health.mil/transformations/2016/8/definitions#DataSet"/>
        <rdfs:range rdf:resource="http://www.w3.org/2001/XMLSchema#dateTime"/>
        <rdfs:comment>
            Indicates the last date/time when this dataset was ingested.
        </rdfs:comment>
    </owl:DatatypeProperty>

    <!-- http://www.semanticweb.org/phoehne/ontologies/2016/8/transformations#predicate -->

    <owl:DatatypeProperty rdf:about="http://dveivr.dha.health.mil/transformations/2016/8/definitions#predicate">
        <rdfs:domain rdf:resource="http://dveivr.dha.health.mil/transformations/2016/8/definitions#IngestTransformation"/>
        <rdfs:range rdf:resource="http://www.w3.org/2001/XMLSchema#anyURI"/>
        <rdfs:comment>
            This is the output predicate value for the triples we&apos;re creating at the end of transformation.
            The subject is the URI of the XML document that&apos;s being ingested and enriched.  This is the predicate
            that connects it to a given value or URI of an entity/class within the ontology.
        </rdfs:comment>
    </owl:DatatypeProperty>

    <!-- http://www.semanticweb.org/phoehne/ontologies/2016/8/transformations#xpath -->

    <owl:DatatypeProperty rdf:about="http://dveivr.dha.health.mil/transformations/2016/8/definitions#xpath">
        <rdfs:domain rdf:resource="http://dveivr.dha.health.mil/transformations/2016/8/definitions#IngestTransformation"/>
        <rdfs:range rdf:resource="http://www.w3.org/2001/XMLSchema#string"/>
        <rdfs:comment>
            This is the XPATH statement that, when executed against the input XML document, will produce a
            raw value that must be translated.
        </rdfs:comment>
    </owl:DatatypeProperty>

    <!-- http://www.semanticweb.org/phoehne/ontologies/2016/8/transformations#xpath -->

    <owl:DatatypeProperty rdf:about="http://dveivr.dha.health.mil/transformations/2016/8/definitions#caseIndpendent">
        <rdfs:domain rdf:resource="http://dveivr.dha.health.mil/transformations/2016/8/definitions#IngestTransformation"/>
        <rdfs:range rdf:resource="http://www.w3.org/2001/XMLSchema#boolean"/>
        <rdfs:comment>
            Indicates if the transformation should be perofrmed in a case indepdent manner.
        </rdfs:comment>
    </owl:DatatypeProperty>

    <!-- -->

    <owl:DatatypeProperty rdf:about="http://dveivr.dha.health.mil/transformations/2016/8/definitions#outputType">
        <rdfs:domain rdf:resource="http://dveivr.dha.health.mil/transformations/2016/8/definitions#Mapping"/>
        <rdfs:range rdf:resource="http://www.w3.org/2001/XMLSchema#string"/>
        <rdfs:comment>When mapping simple values, this is the parent data property type for the values.</rdfs:comment>
    </owl:DatatypeProperty>

    <!-- http://www.semanticweb.org/phoehne/ontologies/2016/8/transformations#transformationValue -->

    <owl:DatatypeProperty rdf:about="http://dveivr.dha.health.mil/transformations/2016/8/definitions#transformationValue">
        <rdfs:domain rdf:resource="http://dveivr.dha.health.mil/transformations/2016/8/definitions#SimpleValueMapping"/>
        <rdfs:comment>When mapping simple values, this is the parent data property type for the values.</rdfs:comment>
    </owl:DatatypeProperty>

    <!-- http://www.semanticweb.org/phoehne/ontologies/2016/8/transformations#inputValue -->

    <owl:DatatypeProperty rdf:about="http://dveivr.dha.health.mil/transformations/2016/8/definitions#inputValue">
        <rdfs:subPropertyOf rdf:resource="http://dveivr.dha.health.mil/transformations/2016/8/definitions#transformationValue"/>
        <rdfs:range rdf:resource="http://www.w3.org/2001/XMLSchema#string"/>
        <rdfs:range rdf:resource="http://www.w3.org/2001/XMLSchema#boolean"/>
        <rdfs:range rdf:resource="http://www.w3.org/2001/XMLSchema#dateTime"/>
        <rdfs:range rdf:resource="http://www.w3.org/2001/XMLSchema#double"/>
        <rdfs:range rdf:resource="http://www.w3.org/2001/XMLSchema#int"/>
        <rdfs:comment>This is the given input value.  This is what is in the source document.</rdfs:comment>
    </owl:DatatypeProperty>
    


    <!-- http://www.semanticweb.org/phoehne/ontologies/2016/8/transformations#outputValue -->

    <owl:DatatypeProperty rdf:about="http://dveivr.dha.health.mil/transformations/2016/8/definitions#outputValue">
        <rdfs:subPropertyOf rdf:resource="http://dveivr.dha.health.mil/transformations/2016/8/definitions#transformationValue"/>
        <rdfs:range rdf:resource="http://www.w3.org/2001/XMLSchema#boolean"/>
        <rdfs:range rdf:resource="http://www.w3.org/2001/XMLSchema#dateTime"/>
        <rdfs:range rdf:resource="http://www.w3.org/2001/XMLSchema#double"/>
        <rdfs:range rdf:resource="http://www.w3.org/2001/XMLSchema#int"/>
        <rdfs:range rdf:resource="http://www.w3.org/2001/XMLSchema#string"/>
        <rdfs:comment>
            This is a simple output value that we would put in the output triples.  For example, when translating the
            input value &quot;2&quot; for gender, this may translate to &quot;Female&quot;.
        </rdfs:comment>
    </owl:DatatypeProperty>
    


    <!-- http://www.semanticweb.org/phoehne/ontologies/2016/8/transformations#subjectUri -->

    <owl:DatatypeProperty rdf:about="http://dveivr.dha.health.mil/transformations/2016/8/definitions#subjectUri">
        <rdfs:subPropertyOf rdf:resource="http://dveivr.dha.health.mil/transformations/2016/8/definitions#transformationValue"/>
        <rdfs:domain rdf:resource="http://dveivr.dha.health.mil/transformations/2016/8/definitions#SimpleValueMapping"/>
        <rdfs:range rdf:resource="http://www.w3.org/2001/XMLSchema#anyURI"/>
        <rdfs:comment>
            When transforming a simple input value this is the output URI.  For example, the translation of the
            value &quot;yes&quot; for a given attribute might be a reference to an instance in the ontology.
        </rdfs:comment>
    </owl:DatatypeProperty>

    <!-- http://www.semanticweb.org/phoehne/ontologies/2016/8/transformations#noInputValue -->

    <owl:DatatypeProperty rdf:about="http://dveivr.dha.health.mil/transformations/2016/8/definitions#noInputValue">
        <rdfs:subPropertyOf rdf:resource="http://dveivr.dha.health.mil/transformations/2016/8/definitions#transformationValue"/>
        <rdfs:domain rdf:resource="http://dveivr.dha.health.mil/transformations/2016/8/definitions#SimpleValueMapping"/>
        <rdfs:range rdf:resource="http://www.w3.org/2001/XMLSchema#anyURI"/>
        <rdfs:comment>
            When transforming a simple input value this is the output URI.  For example, the translation of the
            value &quot;yes&quot; for a given attribute might be a reference to an instance in the ontology.
        </rdfs:comment>
    </owl:DatatypeProperty>

    <!-- http://www.semanticweb.org/phoehne/ontologies/2016/8/transformations#unmappedValue -->

    <owl:DatatypeProperty rdf:about="http://dveivr.dha.health.mil/transformations/2016/8/definitions#unmappedValue">
        <rdfs:subPropertyOf rdf:resource="http://dveivr.dha.health.mil/transformations/2016/8/definitions#transformationValue"/>
        <rdfs:domain rdf:resource="http://dveivr.dha.health.mil/transformations/2016/8/definitions#SimpleValueMapping"/>
        <rdfs:domain rdf:resource="http://dveivr.dha.health.mil/transformations/2016/8/definitions#InvokeTransformMapping"/>
        <rdfs:range rdf:resource="http://www.w3.org/2001/XMLSchema#string"/>
        <rdfs:comment>
            When transforming a simple input value this is the output URI.  For example, the translation of the
            value &quot;yes&quot; for a given attribute might be a reference to an instance in the ontology.
        </rdfs:comment>
    </owl:DatatypeProperty>
    


    <!-- http://www.semanticweb.org/phoehne/ontologies/2016/8/transformations#transformDefaultValue -->

    <owl:DatatypeProperty rdf:about="http://dveivr.dha.health.mil/transformations/2016/8/definitions#transformDefaultValue">
        <rdfs:domain rdf:resource="http://dveivr.dha.health.mil/transformations/2016/8/definitions#PassthroughValueMapping"/>
        <rdfs:domain rdf:resource="http://dveivr.dha.health.mil/transformations/2016/8/definitions#SimpleValueMapping"/>
        <rdfs:range rdf:resource="http://www.w3.org/2001/XMLSchema#anyURI"/>
        <rdfs:range rdf:resource="http://www.w3.org/2001/XMLSchema#boolean"/>
        <rdfs:range rdf:resource="http://www.w3.org/2001/XMLSchema#dateTime"/>
        <rdfs:range rdf:resource="http://www.w3.org/2001/XMLSchema#double"/>
        <rdfs:range rdf:resource="http://www.w3.org/2001/XMLSchema#int"/>
        <rdfs:range rdf:resource="http://www.w3.org/2001/XMLSchema#string"/>
        <rdfs:comment>
            In the case the input value is blank, this is the default value to assign during the transformation process.
        </rdfs:comment>
    </owl:DatatypeProperty>
    


    <!-- http://www.semanticweb.org/phoehne/ontologies/2016/8/transformations#transformModuleFunction -->

    <owl:DatatypeProperty rdf:about="http://dveivr.dha.health.mil/transformations/2016/8/definitions#transformModuleFunction">
        <rdfs:domain rdf:resource="http://dveivr.dha.health.mil/transformations/2016/8/definitions#InvokeTransformMapping"/>
        <rdfs:range rdf:resource="http://www.w3.org/2001/XMLSchema#string"/>
        <rdfs:comment>
            The name of the function in the transformation module.  E.g. the module might have several date utility
            functions and this might be &quot;convertMDYtoYMD&quot;
        </rdfs:comment>
    </owl:DatatypeProperty>
    


    <!-- http://www.semanticweb.org/phoehne/ontologies/2016/8/transformations#transformModuleNamespace -->

    <owl:DatatypeProperty rdf:about="http://dveivr.dha.health.mil/transformations/2016/8/definitions#transformModuleNamespace">
        <rdfs:domain rdf:resource="http://dveivr.dha.health.mil/transformations/2016/8/definitions#InvokeTransformMapping"/>
        <rdfs:range rdf:resource="http://www.w3.org/2001/XMLSchema#anyURI"/>
        <rdfs:comment>This is the namespace of the transformation module.</rdfs:comment>
    </owl:DatatypeProperty>
    


    <!-- http://www.semanticweb.org/phoehne/ontologies/2016/8/transformations#transformModuleUri -->

    <owl:DatatypeProperty rdf:about="http://dveivr.dha.health.mil/transformations/2016/8/definitions#transformModuleUri">
        <rdfs:domain rdf:resource="http://dveivr.dha.health.mil/transformations/2016/8/definitions#InvokeTransformMapping"/>
        <rdfs:range rdf:resource="http://www.w3.org/2001/XMLSchema#anyURI"/>
        <rdfs:comment>This is the URI of the transformation module withing MarkLogic.  E.g. &quot;/ext/transforms/date-transforms.xqy&quot;</rdfs:comment>
    </owl:DatatypeProperty>

    <!-- http://www.semanticweb.org/phoehne/ontologies/2016/8/transformations#transformModuleUri -->

    <owl:DatatypeProperty rdf:about="http://dveivr.dha.health.mil/transformations/2016/8/definitions#parameterName">
        <rdfs:domain rdf:resource="http://dveivr.dha.health.mil/transformations/2016/8/definitions#Parameter"/>
        <rdfs:range rdf:resource="http://www.w3.org/2001/XMLSchema#string"/>
        <rdfs:comment>
            This is the parameter name.
        </rdfs:comment>
    </owl:DatatypeProperty>

    <!-- http://www.semanticweb.org/phoehne/ontologies/2016/8/transformations#transformModuleUri -->

    <owl:DatatypeProperty rdf:about="http://dveivr.dha.health.mil/transformations/2016/8/definitions#parameterValue">
        <rdfs:domain rdf:resource="http://dveivr.dha.health.mil/transformations/2016/8/definitions#Parameter"/>
        <rdfs:range rdf:resource="http://www.w3.org/2001/XMLSchema#anyURI"/>
        <rdfs:range rdf:resource="http://www.w3.org/2001/XMLSchema#boolean"/>
        <rdfs:range rdf:resource="http://www.w3.org/2001/XMLSchema#dateTime"/>
        <rdfs:range rdf:resource="http://www.w3.org/2001/XMLSchema#double"/>
        <rdfs:range rdf:resource="http://www.w3.org/2001/XMLSchema#int"/>
        <rdfs:range rdf:resource="http://www.w3.org/2001/XMLSchema#string"/>
        <rdfs:comment>
            This is the parameter value.
        </rdfs:comment>
    </owl:DatatypeProperty>


</rdf:RDF>
